SkLean/Typing2.lean
@@ -43,33 +43,112 @@ end valid_judgment_weak
 
 inductive has_final_judgment : Expr → Expr → Prop
   | trivial : valid_judgment_weak e t → has_final_judgment e t
-  | hard    : is_eval_once t t'       → has_final_judgment e t' → has_final_judgment e t
+  | hard    : beta_eq t t'            → has_final_judgment e t' → has_final_judgment e t
 
 namespace has_final_judgment
+
+lemma imp_valid_judgment (e : Expr) : has_final_judgment e t → valid_judgment e t := by
+  intro h
+  induction h
+  case trivial _ _ h =>
+    exact h.weakening
+  case hard t' t'' e' h_step h_t' ih =>
+    apply valid_judgment.step_beta_eq
+    exact ih
+    apply beta_eq.symm
+    exact h_step
+
+lemma imp_m : has_final_judgment e t → has_final_judgment e SKM[((M e.max_universe.succ) e)] := by
+  intro h
+  induction h
+  case trivial e' t' h =>
+    apply has_final_judgment.hard
+    apply beta_eq.eval
+    apply is_eval_once.m
+    exact h.weakening
+    exact has_final_judgment.trivial h
+  case hard t' t'' e' h_eval_step h_t' ih =>
+    exact ih
 
 lemma preserved : has_final_judgment e t → is_eval_once e e' → has_final_judgment e' t := by
   intro h_t h_eval
   induction h_t
   case trivial e'' t' h =>
-    apply valid_judgment_weak.eval_preserves_judgment_hard at h
-    apply has_final_judgment.trivial
-    exact h h_eval
-  case hard t'' t''' e'' h_eval' h_final h_step =>
+    cases e'
+    case m m =>
+      match m with
+        | .mk n =>
+          apply has_final_judgment.trivial at h
+          apply has_final_judgment.hard
+          apply beta_eq.symm
+          apply beta_eq.eval
+          apply is_eval_once.m
+          use (Expr.m m).max_universe.succ
+          apply h.imp_valid_judgment
+          apply has_final_judgment.hard
+          apply beta_eq.right
+          apply beta_eq.eval
+          exact h_eval
+          apply has_final_judgment.hard
+          apply beta_eq.eval
+          apply is_eval_once.m
+          apply valid_judgment.m
+          apply has_final_judgment.trivial
+          apply valid_judgment_weak.m
+    case k k =>
+      match k with
+        | .mk n =>
+          apply has_final_judgment.trivial at h
+          apply has_final_judgment.hard
+          apply beta_eq.symm
+          apply beta_eq.eval
+          apply is_eval_once.m
+          use (Expr.k k).max_universe.succ
+          apply h.imp_valid_judgment
+          apply has_final_judgment.hard
+          apply beta_eq.right
+          apply beta_eq.eval
+          exact h_eval
+          apply has_final_judgment.hard
+          apply beta_eq.eval
+          apply is_eval_once.m
+          apply valid_judgment.k
+          apply has_final_judgment.trivial
+          apply valid_judgment_weak.k
+    case s s =>
+      match s with
+        | .mk n =>
+          apply has_final_judgment.trivial at h
+          apply has_final_judgment.hard
+          apply beta_eq.symm
+          apply beta_eq.eval
+          apply is_eval_once.m
+          use (Expr.s s).max_universe.succ
+          apply h.imp_valid_judgment
+          apply has_final_judgment.hard
+          apply beta_eq.right
+          apply beta_eq.eval
+          exact h_eval
+          apply has_final_judgment.hard
+          apply beta_eq.eval
+          apply is_eval_once.m
+          apply valid_judgment.s
+          apply has_final_judgment.trivial
+          apply valid_judgment_weak.s
+    case call c =>
+      match c with
+        | .mk lhs rhs =>
+          cases h
+          cases h_eval
+          cases h_eval
+          cases h_eval
+          case call lhs' rhs' h_u h_t_lhs h_t_rhs =>
+            cases h_t_lhs
+  case hard t'' t''' e' h_beq h_t' ih =>
     simp_all
     apply has_final_judgment.hard
-    exact h_eval'
-    exact h_step
-
-lemma imp_valid_judgment : has_final_judgment e t → valid_judgment e t := by
-  intro h
-  induction h
-  case trivial h =>
-    apply valid_judgment_weak.weakening
-    exact h
-  case hard t'' t''' e' h_t_eq h_t h_t'' =>
-    apply valid_judgment.step_beta_eq
-    exact h_t''
-    exact h_t_eq
+    exact h_beq
+    exact ih
 
 lemma imp_exists_valid_judgment_weak : has_final_judgment e t → ∃ t, valid_judgment_weak e t := by
   intro h
@@ -96,13 +175,12 @@ lemma imp_has_final_judgment : valid_judgment e t → has_final_judgment e t := 
     apply has_final_judgment.trivial
     apply valid_judgment_weak.m
   case call lhs rhs h_u h_t_lhs h_t_rhs =>
-    apply has_final_judgment.hard
-    
-    exact h_u
+    apply has_final_judgment.trivial at h_t_lhs
+    apply has_final_judgment.trivial at h_t_lhs
+    sorry
+  case step_beta_eq t' h_t =>
     
     sorry
-  case step_beta_eq t' h_t
-  sorry
 
 theorem preserved : valid_judgment e t → is_eval_once e e' → valid_judgment e' t := by
   intro h_t h_eval
